tests/lean/run/matchArrayLit.lean
@@ -1,0 +1,79 @@
+universes u v
+
+theorem eqLitOfSize0 {α : Type u} (a : Array α) (hsz : a.size = 0) : a = #[] :=
+a.toArrayLitEq 0 hsz
+
+theorem eqLitOfSize1 {α : Type u} (a : Array α) (hsz : a.size = 1) : a = #[a.getLit 0 hsz (ofDecideEqTrue rfl)] :=
+a.toArrayLitEq 1 hsz
+
+theorem eqLitOfSize2 {α : Type u} (a : Array α) (hsz : a.size = 2) : a = #[a.getLit 0 hsz (ofDecideEqTrue rfl), a.getLit 1 hsz (ofDecideEqTrue rfl)] :=
+a.toArrayLitEq 2 hsz
+
+theorem eqLitOfSize3 {α : Type u} (a : Array α) (hsz : a.size = 3) :
+  a = #[a.getLit 0 hsz (ofDecideEqTrue rfl), a.getLit 1 hsz (ofDecideEqTrue rfl), a.getLit 2 hsz (ofDecideEqTrue rfl)] :=
+a.toArrayLitEq 3 hsz
+
+/-
+Matcher for the following patterns
+```
+| #[]           => _
+| #[a₁]         => _
+| #[a₁, a₂, a₃] => _
+| a             => _
+``` -/
+def matchArrayLit {α : Type u} (C : Array α → Sort v) (a : Array α)
+    (h₁ : Unit →      C #[])
+    (h₂ : ∀ a₁,       C #[a₁])
+    (h₃ : ∀ a₁ a₂ a₃, C #[a₁, a₂, a₃])
+    (h₄ : ∀ a,        C a)
+    : C a :=
+if h : a.size = 0 then
+  @Eq.rec _ _ (fun x _ => C x) (h₁ ()) _ (a.toArrayLitEq 0 h).symm
+else if h : a.size = 1 then
+  @Eq.rec _ _ (fun x _ => C x) (h₂ (a.getLit 0 h (ofDecideEqTrue rfl))) _ (a.toArrayLitEq 1 h).symm
+else if h : a.size = 3 then
+  @Eq.rec _ _ (fun x _ => C x) (h₃ (a.getLit 0 h (ofDecideEqTrue rfl)) (a.getLit 1 h (ofDecideEqTrue rfl)) (a.getLit 2 h (ofDecideEqTrue rfl))) _ (a.toArrayLitEq 3 h).symm
+else
+  h₄ a
+
+/- Equational lemmas that should be generated automatically. -/
+theorem matchArrayLit.eq1 {α : Type u} (C : Array α → Sort v)
+    (h₁ : Unit →      C #[])
+    (h₂ : ∀ a₁,       C #[a₁])
+    (h₃ : ∀ a₁ a₂ a₃, C #[a₁, a₂, a₃])
+    (h₄ : ∀ a,        C a)
+    : matchArrayLit C #[] h₁ h₂ h₃ h₄ = h₁ () :=
+rfl
+
+theorem matchArrayLit.eq2 {α : Type u} (C : Array α → Sort v)
+    (h₁ : Unit →      C #[])
+    (h₂ : ∀ a₁,       C #[a₁])
+    (h₃ : ∀ a₁ a₂ a₃, C #[a₁, a₂, a₃])
+    (h₄ : ∀ a,        C a)
+    (a₁ : α)
+    : matchArrayLit C #[a₁] h₁ h₂ h₃ h₄ = h₂ a₁ :=
+rfl
+
+theorem matchArrayLit.eq3 {α : Type u} (C : Array α → Sort v)
+    (h₁ : Unit →      C #[])
+    (h₂ : ∀ a₁,       C #[a₁])
+    (h₃ : ∀ a₁ a₂ a₃, C #[a₁, a₂, a₃])
+    (h₄ : ∀ a,        C a)
+    (a₁ a₂ a₃ : α)
+    : matchArrayLit C #[a₁, a₂, a₃] h₁ h₂ h₃ h₄ = h₃ a₁ a₂ a₃ :=
+rfl
+
+theorem matchArrayLit.eq4 {α : Type u} (C : Array α → Sort v)
+    (h₁ : Unit →      C #[])
+    (h₂ : ∀ a₁,       C #[a₁])
+    (h₃ : ∀ a₁ a₂ a₃, C #[a₁, a₂, a₃])
+    (h₄ : ∀ a,        C a)
+    (a : Array α)
+    (n₁ : a.size ≠ 0) (n₂ : a.size ≠ 1) (n₃ : a.size ≠ 3)
+    : matchArrayLit C a h₁ h₂ h₃ h₄ = h₄ a :=
+match a, n₁, n₂, n₃ with
+| ⟨0, _⟩,   n₁, _, _  => absurd rfl n₁
+| ⟨1, _⟩,   _,  n₂, _ => absurd rfl n₂
+| ⟨2, _⟩,   _, _, _   => rfl
+| ⟨3, _⟩,   _, _, n₃  => absurd rfl n₃
+| ⟨n+4, _⟩, _, _, _   => rfl
